proof of runb and state_to_list_cons

code/rocq/elpi.v
@@ -101,6 +101,22 @@ Module Nur (U : Unif).
   Lemma add_altsbagliate_emptyr {l}: add_altsbagliata l [::] = [::].
   Proof. rewrite /add_altsbagliata/=flatten_empty//. Qed.
 
+  (* Dead /\ A = Dead, Dead \/ A = A
+  Fixpoint clean_dead (A : state) : state :=
+    match A with
+    | OK | Top | Bot | Dead | Goal _ _ => A
+    | And A B0 B =>
+        match clean_dead A with
+        | Dead => Dead
+        | A' => And A' B0 (clean_dead B)
+        end
+    | Or A sB B =>
+        match clean_dead A with
+        | Dead => clean_dead B (* bug: B goes with sB !!!! *)
+        | A' => Or A' sB (clean_dead B)
+        end
+    end. *)
+
   Fixpoint state_to_list (A: state) (bt : list alt) : list alt :=
     match A with
       (* Attenzione: bisogna tradurre: "Dead /\ p" che è diverso da "OK /\ p", quindi è strano
@@ -137,133 +153,645 @@ Module Nur (U : Unif).
       add_alt lB0 lA lB
     end.
 
-  Goal forall p x y z w s1 s2 a, 
-    let f x := (Goal p (Call x)) in
-    state_to_list (
-      And 
-        (Or (f x) s1 (f y)) (f a) 
-        (Or (f z) s2 (f w))) [::] = 
-      [:: [:: call x; call z];
-      [:: call x; call w];
-      [:: call y; call a]].
-  Proof.
-    move=>/=.
-    by [].
-  Qed.
+  Section tests.
+    Goal forall p x y z w s1 s2 a, 
+      let f x := (Goal p (Call x)) in
+      state_to_list (
+        And 
+          (Or (f x) s1 (f y)) (f a) 
+          (Or (f z) s2 (f w))) [::] = 
+        [:: [:: call x; call z];
+        [:: call x; call w];
+        [:: call y; call a]].
+    Proof.
+      move=>/=.
+      by [].
+    Qed.
 
-  Goal forall p z w s1 s2 a, 
-    let f x := (Goal p (Call x)) in
-    state_to_list (
-      And 
-        (Or Top s1 Bot) (f a) 
-        (Or (f z) s2 (f w))) [::] = 
-      [:: [:: call z]; [:: call w]].
-  Proof.
-    move=>/=.
-    by [].
-  Qed.
+    Goal forall p z w s1 s2 a, 
+      let f x := (Goal p (Call x)) in
+      state_to_list (
+        And 
+          (Or Top s1 Bot) (f a) 
+          (Or (f z) s2 (f w))) [::] = 
+        [:: [:: call z]; [:: call w]].
+    Proof.
+      move=>/=.
+      by [].
+    Qed.
 
-  (* THIS IS IMPORTANT *)
-  Goal forall p s1 s2 a b c d, 
-    let f x := (Goal p (Call x)) in
-    state_to_list (
-      And 
-        (Or Bot s1 (f a)) (f b) 
-        (Or (f c) s2 (f d))) [::] = 
-      (* [:: [:: call a; call b] ]. *)
-      [:: [:: call a; call c]; [::call a; call d] ].
-  Proof.
-    move=> p s1 s2 a b c d /=.
-    by [].
-  Qed.
+    (* THIS IS IMPORTANT *)
+    Goal forall p s1 s2 a b c d, 
+      let f x := (Goal p (Call x)) in
+      state_to_list (
+        And 
+          (Or Bot s1 (f a)) (f b) 
+          (Or (f c) s2 (f d))) [::] = 
+        (* [:: [:: call a; call b] ]. *)
+        [:: [:: call a; call c]; [::call a; call d] ].
+    Proof.
+      move=> p s1 s2 a b c d /=.
+      by [].
+    Qed.
 
-  Goal forall p a b s1 s2, 
-    state_to_list (
-      Or 
-        (Or (Goal p Cut) s1 (Goal p (Call a))) s2
-        (Goal p (Call b))) [::] = 
-     [:: [:: cut [:: [:: call b]]]; [:: call a]; [:: call b]].
-  Proof. by []. Qed.
+    Goal forall p a b s1 s2, 
+      state_to_list (
+        Or 
+          (Or (Goal p Cut) s1 (Goal p (Call a))) s2
+          (Goal p (Call b))) [::] = 
+      [:: [:: cut [:: [:: call b]]]; [:: call a]; [:: call b]].
+    Proof. by []. Qed.
 
-  Goal forall b0 p a b c s1 s2, 
-    state_to_list (
-      Or 
-        (Or (And (Goal p (Call c)) b0 (Goal p Cut)) s1 (Goal p (Call a))) s2
-        (Goal p (Call b))) [::] = 
-     [:: [:: call c; cut [:: [:: call b]]]; [:: call a]; [:: call b]].
-  Proof. by []. Qed.
+    Goal forall A1 A2 s  C0 B p,
+      let f x := (Goal p (Call x)) in
+      state_to_list (And (Or (f A1) s (f A2)) (Bot) (And Bot (f C0) (f B))) [::] =
+      [:: ].
+    Proof.
+      move=> * /=.
+      by [].
+    Qed.
+
+    Goal forall A1 A2 s B0 C0 B p,
+      let f x := (Goal p (Call x)) in
+      state_to_list (And (Or (f A1) s (f A2)) (f B0) (And Bot (f C0) (f B))) [::] =
+      [:: [:: call A2 ; call B0 ]].
+    Proof.
+      move=> * /=.
+      by [].
+    Qed.
+
+    Goal forall b0 p a b c s1 s2, 
+      state_to_list (
+        Or 
+          (Or (And (Goal p (Call c)) b0 (Goal p Cut)) s1 (Goal p (Call a))) s2
+          (Goal p (Call b))) [::] = 
+      [:: [:: call c; cut [:: [:: call b]]]; [:: call a]; [:: call b]].
+    Proof. by []. Qed.
+
+  End tests.
 
   Definition state_to_list_cons A :=
     forall l, exists x xs, state_to_list A l = x :: xs.
-
-  Definition nur' A l s s1 r1 :=
-    forall x xs, state_to_list A l = x :: xs ->
-        forall p, nur p s x xs s1 r1.
 
   Definition runElpi A :=
     forall s B s1 b,
       valid_state A ->
         runb s A s1 B b -> 
-          forall l, exists r1, nur' A l s s1 r1 /\ state_to_list B l = r1.
+          forall l p, exists x xs, state_to_list A l = x :: xs /\ nur p s x xs s1 (state_to_list B l).
+    
 
-  (* Goal forall p z w a, 
-    let f x := (Goal p (Call x)) in
-    runElpi (
-    And 
-      (Or OK empty (Or Bot empty Bot)) (And (f a) Top Top) 
-      (Or (f z) empty (Or Bot empty (And (f w) Top Top)))).
-  Proof.
-    rewrite /runElpi => p z w a s B0 s1 b.
-    rewrite /valid_state.
-    simpl is_dead.
-    rewrite /bbAnd.
-    simpl base_and.
-    simpl orb.
-    rewrite /bbOr.
-    simpl base_or_aux.
-    simpl success.
-    simpl base_or_aux_ko.
-    simpl orb.
-    simpl.
-    simpl base_and_ko.
-    move=>/=.
-    rewrite if_same.
-    move=> p z w a//. *)
-
-
-  Goal @runElpi OK.
-  Proof.
-    rewrite/runElpi/nur' => s B s1 b _ H.
-    inversion H; clear H; subst => //=; inversion H0 => //p; subst.
-    case: H6 => <- <-/=.
-    eexists; split; [|reflexivity].
-    move=> ??[<-<-]?.
-    apply: StopE.
-  Qed.
-  
-  Goal @runElpi Bot.
-  Proof.
-    rewrite /runElpi/nur' => s B s1 b _ H.
-    inversion H; clear H => //; subst => /=.
-      inversion H0 => //.
-    inversion H0; clear H0; subst => //.
-    inversion H6; clear H6; subst => //.
-  Qed.
-  
-  Goal @runElpi Top.
-  Proof.
-    rewrite/runElpi/nur' => s B s1 b _ H.
-    inversion H; subst => //=.
-    - inversion H0; subst => //.
-      case: H1 => ??; subst.
-      inversion H2; subst => //.
-      case: H7 => ??; subst => /=.
-      eexists; split => //??[<-<-]?.
+  Section tests.
+    Goal @runElpi OK.
+    Proof.
+      rewrite/runElpi => s B s1 b _ H.
+      inversion H; clear H; subst => //=; inversion H0 => //p; subst.
+      case: H6 => <- <-/=.
+      exists [::], [::]; split => //.
       apply: StopE.
-    - inversion H0; subst => //.
-      case: H3 => ??;subst.
-      inversion H4 => //.
-  Qed.
+    Qed.
+    
+    Goal @runElpi Bot.
+    Proof.
+      rewrite /runElpi => s B s1 b _ H.
+      inversion H; clear H => //; subst => /=.
+      inversion H0 => //.
+      inversion H0; clear H0; subst => //.
+      inversion H6; clear H6; subst => //.
+    Qed.
+    
+    Goal @runElpi Top.
+    Proof.
+      rewrite/runElpi => s B s1 b _ H.
+      inversion H; subst => //=.
+      - inversion H0; subst => //.
+        case: H1 => ??; subst.
+        inversion H2; subst => //.
+        case: H7 => ??; subst => /=.
+        exists [::], [::]; split => //.
+        apply: StopE.
+      - inversion H0; subst => //.
+        case: H3 => ??;subst.
+        inversion H4 => //.
+    Qed.
+  End tests.
+
+  Section state_to_list_prop.
+    Lemma state_to_list_dead {A l}: is_dead A -> state_to_list A l = [::].
+    Proof.
+      elim: A l => //.
+      - move=> A HA s B HB/= l/andP[dA dB].
+        rewrite HB// HA//.
+      - move=> A HA B0 HB0 B HB l /=dA.
+        rewrite HA//=.
+    Qed.
+  End state_to_list_prop.
+
+  Section list_cons.
+
+    Lemma success_state_to_list {A m}:
+      success A ->
+        state_to_list A m = [::] :: (state_to_list (clean_success A) m).
+    Proof.
+      elim: A m => //.
+      - move=> A HA s B HB/= m.
+        case: ifP => [dA sB|dA sA].
+          rewrite (state_to_list_dead dA)/=.
+          have:= HB _ sB=>->.
+          rewrite (state_to_list_dead dA)//=.
+        have:= HA (state_to_list B m ++ m) sA.
+        move=>->//.
+      - move=> A HA B0 HB0 B HB m /=/andP[sA sB].
+        rewrite /add_alt sA=>/=.
+        have:= HA m sA => ->.
+        have:= HB m sB => ->//=.
+    Qed.
+
+    Lemma expand_solved_state_to_list_same {s1 A s2 B l}:
+      expand s1 A = Solved s2 B -> state_to_list A l = state_to_list B l.
+    Proof.
+      elim: A s1 B s2 l => //.
+      - move=> /= ????[_<-]//.
+      - move=>?[]//.
+      - move=> A HA s B HB s1 C s2 l.
+        move=>/simpl_expand_or_solved[].
+          move=>[A'[HA'->]]/=.
+          by rewrite (HA _ _ _ _ HA').
+        move=> [B'[dA[HB' ->]]]/=.
+        rewrite !(state_to_list_dead dA)//=.
+        apply: HB HB'.
+      - move=> A HA B0 _ B HB s1 C s2 l.
+        move=>/simpl_expand_and_solved[s'[A'[B'[HA'[HB'->]]]]]/=.
+        by rewrite (HA _ _ _ _ HA')(HB _ _ _ _ HB').
+    Qed.
+
+    Lemma state_to_list_empty_clean {B l}:
+      success B -> state_to_list B l = [::[::]] ->
+        state_to_list (clean_success B) l = [::].
+    Proof.
+      move=>/success_state_to_list->.
+      by move=>[].
+    Qed.
+
+    Lemma state_to_list_eq_clean {A B l}:
+      success A -> success B -> state_to_list A l = state_to_list B l ->
+        state_to_list (clean_success A) l = state_to_list (clean_success B) l.
+    Proof.
+      move=>/success_state_to_list->.
+      by move=>/success_state_to_list->[].
+    Qed.
+
+    Lemma base_and_state_to_list {A}: base_and A -> state_to_list_cons A.
+    Proof.
+      elim: A => //=.
+      - by do 2 eexists.
+      - move=> []//p [|t]//= _ B0 _ B HB/andP[/eqP->/HB] H l; have[x[xs]]:= H l => /=->; by do 2 eexists.
+    Qed.
+
+    Lemma base_and_ko_state_to_list {A l}: base_and_ko A -> state_to_list A l = [::].
+    Proof. elim: A => //=-[]//. Qed.
+
+    Lemma base_or_aux_ko_state_to_list {A l}: base_or_aux_ko A -> state_to_list A l = [::].
+    Proof.
+      elim: A l => //.
+      - move=> /= A HA s B HB l /andP[bA bB]; rewrite HB//=base_and_ko_state_to_list//.
+      - move=>[]//.
+    Qed.
+
+    Lemma failed_state_to_list {A}:
+      valid_state A -> failed A = false -> state_to_list_cons A.
+    Proof.
+      elim: A => //.
+      - move=> /=. by move=> /=; do 2 eexists.
+      - by move=> /=; do 2 eexists.
+      - by move=> p []//=; do 2 eexists.
+      - move=> A HA s B HB/=++l.
+        case: ifP => [dA vB fB|dA /andP[vA bB] fA]/=.
+          rewrite (state_to_list_dead dA).
+          apply: HB => //.
+        have [x[xs ->]] := HA vA fA (state_to_list B l ++ l).
+        by do 2 eexists.
+      - move=> A HA B0 _ B HB/= /and3P[]++++l/=.
+        case: ifP => [sA vA vB bB0|sA vA/eqP->]/=.
+          rewrite success_failed//==>fB.
+          rewrite (success_state_to_list sA)/=.
+          have [x[xs]]:= HB vB fB l.
+          move=>->/=; by do 2 eexists.
+        rewrite orbF => + fA; rewrite fA => bB.
+        have [x[xs ->]]:= HA vA fA l.
+        have [y[ys ->]]:= base_and_state_to_list bB l.
+        by do 2 eexists.
+    Qed.
+
+    Lemma next_alt_state_to_list_old {s1 A s2 B}:
+      valid_state A -> next_alt s1 A = Some (s2, B) -> state_to_list_cons B.
+    Proof.
+      move=>vA H.
+      have:= next_alt_failed H.
+      have:= valid_state_next_alt vA H.
+      apply: failed_state_to_list.
+    Qed.
+
+    Lemma success_next_alt_state_to_list {s1 A}:
+      valid_state A -> success A -> next_alt s1 A = None -> 
+        forall l, exists x, state_to_list A l = [::x].
+    Proof.
+      elim: A s1 => //.
+      - by exists [::].
+      - move=> A HA s B HB s1/=.
+        case: ifP => [dA vB sB|dA /andP[vA bB] sA] + l.
+          rewrite state_to_list_dead//=.
+          case X: next_alt => [[]|]// _.
+          by have:= HB _ vB sB X l.
+        case X: next_alt => [[]|]//.
+        have H:= bbOr_valid bB.
+        case: ifP => dB.
+          rewrite valid_state_dead// in H.
+        (* case: ifP => // fB. *)
+        case Y: next_alt => [[]|]// _.
+        have [x H1] := HA _ vA sA X (state_to_list B l ++ l).
+        rewrite H1/=.
+        have:= bB; rewrite /bbOr.
+        case Z: base_or_aux => //=.
+          have H2 := next_alt_aux_base_or_none Z Y.
+          by subst.
+        move=> bB0'.
+        rewrite (base_or_aux_ko_state_to_list bB0')/=.
+        by eexists.
+      - move=> A HA B0 _ B HB s1 /=/and3P[vA].
+        case: ifP => //sA vB/=bB0 sB + l.
+        rewrite success_is_dead// success_failed//.
+        case X: next_alt => [[]|]//.
+        have [x H1] := HB _ vB sB X l; rewrite H1.
+        case Y: next_alt => [[s2 C]|]//.
+          move: bB0; rewrite /bbAnd.
+          case Z: base_and => //=.
+            rewrite base_and_failed//.
+          move=> bB0; rewrite base_and_ko_failed//base_and_ko_state_to_list/add_alt//=.
+          rewrite success_state_to_list//flatten_empty.
+          by eexists.
+        have [y H2] := HA _ vA sA Y l.
+        rewrite H2/=; by eexists.
+    Qed.
+
+    Lemma bbOr_next_alt_none {s B l}:
+      bbOr B -> next_alt s B = None -> state_to_list B l = [::].
+    Proof.
+      elim: B s l => //.
+      - move=> A HA s B HB s1 l/=; rewrite /bbOr/=.
+        move=>/orP[]/andP[bA bB].
+          rewrite base_and_dead// next_alt_aux_base_and//.
+        rewrite base_and_ko_is_dead// base_or_aux_is_dead//.
+        have H1 := @next_alt_aux_base_or_ko _ s bB.
+        have H2 :=  @next_alt_aux_base_and_ko _ s1 bA.
+        rewrite (HA _ _ _ H2)// ?(HB _ _ _ H1)///bbOr ?bB?orbT//base_and_ko_base_or_aux_ko//orbT//.
+      - move=> []//p a _ B0 _ B HB s l/=; rewrite /bbOr/=orbF => /andP[/eqP->bB].
+        rewrite next_alt_aux_base_and//.
+    Qed.
+
+    Lemma base_or_aux_next_alt_some {s B s1 D l}:
+      base_or_aux B -> next_alt s B = Some (s1, D) -> state_to_list B l = state_to_list D l.
+    Proof.
+      elim: B s s1 D l => //.
+      - move=>/=???? _[_<-]//.
+      - move=> A HA s B HB s1 s3 C l/=/andP[bA bB].
+        rewrite base_and_dead//next_alt_aux_base_and//.
+        move=>[_<-]//.
+      - move=> []// p a _ B0 _ B HB s1 s2 C l/=/andP[/eqP->bB].
+        rewrite next_alt_aux_base_and// => -[_<-]//.
+    Qed.
+
+
+    Lemma failed_next_alt_state_to_list {s1 A}:
+      valid_state A -> failed A -> next_alt s1 A = None -> 
+        forall l, state_to_list A l = [::].
+    Proof.
+      elim: A s1 => //.
+      - move=> A HA s B HB s1 /=.
+        case: ifP => [dA vB fB|dA /andP[vA bB] fA].
+          case X: next_alt => [[s2 C]|]//.
+          move=> _ l; rewrite (HB s1)//= state_to_list_dead//.
+        case X: next_alt => [[s2 C]|]//.
+        case: ifP => dB.
+          move=>_ l; rewrite (HA s1)//state_to_list_dead//.
+        (* case: ifP => fB//. *)
+        case Y: next_alt => [[]|]// _ l.
+        rewrite (HA s1)//=.
+        rewrite (bbOr_next_alt_none bB Y)//.
+      - move=> A HA B0 HB0 B HB s1/=/and3P[vA].
+        case: ifP => /=[sA vB bB0|sA/eqP->].
+          rewrite success_failed//=success_is_dead// => fB.
+          case X: next_alt => [[]|]//.
+          case Y: next_alt => [[s2 C]|]//.
+            case: ifP => fB0// _ l.
+            rewrite (HB s1)//.
+            have:= bB0; rewrite /bbAnd.
+            case Z: base_and => //=.
+              rewrite base_and_failed// in fB0.
+            move=> bB0'.
+            have H := @next_alt_aux_base_and_ko _ empty bB0'.
+            have H1:= bbAnd_valid bB0.
+            rewrite (HB0 empty)/add_alt//=; case: state_to_list => //*; rewrite flatten_empty//.
+          move=> _ l.
+          have [x H]:= success_next_alt_state_to_list vA sA Y l.
+          rewrite H.
+          rewrite (HB s1)/add_alt//=.
+        case: ifP => //fA bB _ + l.
+        case: ifP => //dA.
+          rewrite (state_to_list_dead dA)//.
+        case X: next_alt => [[s2 C]|].
+          case:ifP => fB => //.
+          have:= bB; rewrite /bbAnd.
+          case Z: base_and => //=.
+            rewrite base_and_failed// in fB.
+          move=> bB0'.
+          have H := @next_alt_aux_base_and_ko _ empty bB0'.
+          have H1:= bbAnd_valid bB.
+          rewrite (HB empty)/add_alt//=; case: state_to_list => //*; rewrite flatten_empty//.
+        have -> //:= HA _ vA fA X l.
+    Qed.
+
+    Lemma expand_state_to_list_cons {s A r}:
+      valid_state A -> expand s A = r -> ~ (is_fail r) -> state_to_list_cons A.
+    Proof. case: r => //[s1 B|s1 B|s1 B]vA H _; apply: failed_state_to_list vA (expand_not_failed H notF). Qed.
+
+    Lemma expandb_done_state_to_list_cons {s A s1 B b}:
+      valid_state A -> expandedb s A (Done s1 B) b -> state_to_list_cons A.
+    Proof.
+      move=> vA /expandedb_Done_not_failed; apply: failed_state_to_list vA.
+    Qed.
+
+    Lemma state_to_list_same_size {r1 r2 A l1 l2}: state_to_list A l1 = r1 -> state_to_list A l2 = r2 -> size r1 = size r2.
+    Proof.
+      move=><-<-; clear.
+      elim: A l1 l2 => //.
+      - move=> A HA s B HB/=l1 l2.
+        rewrite 2!size_cat 2!size_map (HB l1 l2) (HA (state_to_list B l1 ++ l1) (state_to_list B l2 ++ l2))//.
+      - move=> A HA B0 HB0 B HB l1 l2/=.
+        have:= HA l1 l2.
+        case X: (state_to_list A) => [|x xs]//; case Y: state_to_list => [|y ys]//=.
+        rewrite 2!size_cat 2!size_map (HB l1 l2)=>-[H1]; f_equal.
+        have:= HB0 l1 l2.
+        case Z: state_to_list => [|z zs]; case W: state_to_list => [|w ws]//=.
+          rewrite 2!flatten_empty//.
+        move: H1 => + [].
+        clear.
+        elim: xs ys z zs w ws.
+          move=> []//.
+        move=> x xs IH []//y ys/= z zs w ws [] H1 H2.
+        f_equal.
+        rewrite 2!size_cat 2!size_map H2; f_equal.
+        apply: IH => //.
+    Qed.
+
+    Lemma state_to_list_empty_bt {A l1 l2}: state_to_list A l1 = [::] -> state_to_list A l2 = [::].
+    Proof. move=>/state_to_list_same_size => /(_ _ l2 erefl); case: state_to_list => //. Qed.
+
+    Lemma state_to_list_fail {A s A'}:
+      valid_state A ->
+      expand s A = Failure A' -> state_to_list_cons A' ->
+        state_to_list_cons A.
+    Proof.
+      elim: A s A' => //; try by move=> /= _ _ _ [<-]//.
+      - move=>/= p []//.
+      - move=> A HA s B HB s' C/=.
+        case: ifP => //[dA vB|dA /andP[vA bB]] + + l/=.
+          rewrite state_to_list_dead//=.
+          case X: expand => //[D][<-] H1.
+          apply: HB vB X _ _ => l1.
+          have [x[xs/=]] := H1 l1.
+          rewrite state_to_list_dead//= => ->.
+          by do 2 eexists.
+        case X: expand => //[A'][<-] H1.
+        case Z: (state_to_list B) => /=.
+          have H : state_to_list_cons A'.
+            move=> l1; have [y[ys/=]]:= H1 l1.
+            rewrite (state_to_list_empty_bt Z)/=cats0.
+            case: state_to_list => //; by do 2 eexists.
+          have [x[xs->]]:= HA _ _ vA X H l.
+          by do 2 eexists.
+        by case: state_to_list; do 2 eexists.
+      - move=> A HA B0 _ B HB s C /=/and3P[vA].
+        case X: expand => //[A'|s' A'].
+          rewrite (expand_not_solved_not_success X erefl)/=(expand_failure_failed X).
+          move=> /eqP -> + [<-] + l/=.
+          rewrite /bbAnd; case Y: base_and_ko.
+            move=> _ /(_ l)/=; rewrite (base_and_ko_state_to_list Y).
+            case Z: state_to_list => //=; rewrite ?flatten_empty => -[?[]]//.
+          rewrite orbF => bB H.
+          have [x[xs->]]:= base_and_state_to_list bB l.
+          have H1 : state_to_list_cons A'.
+            move=> l1; have [y[ys]]:= H l1 => /=.
+            case: (state_to_list A') => //; by do 2 eexists.
+          have [y[ys->]] := HA _ _ vA X H1 l; by do 2 eexists.
+        rewrite (expand_solved_success X)//==> vB bB0.
+        case Y: expand => //[B'][<-] H l/=.
+        have /= [y[ys H2]] := failed_state_to_list vA (success_failed _ (expand_solved_success X).1) l.
+        rewrite H2/=.
+        have [z[zs]]:= H l => /=.
+        rewrite -(expand_solved_state_to_list_same X) H2/=.
+        case W: state_to_list => [|w ws].
+          move=> /=->; case: state_to_list; by do 2 eexists.
+        have H3: state_to_list_cons B'.
+          move=> l1.
+          have:= state_to_list_same_size W erefl => /(_ l1).
+          case: state_to_list => //; by do 2 eexists.
+        have [b[bs->]]:= HB _ _ vB Y H3 l.
+        by do 2 eexists.
+      Qed.
+
+    Lemma success_success_singleton_next_alt {A l x s}: 
+      success A -> valid_state A ->
+        state_to_list A l = [:: x] -> next_alt s A  = None.
+    Proof.
+      elim: A l x s=> //.
+      - move=> A HA s B HB l x s1/=.
+        case: ifP => //[dA sB vB|dA sA /andP[vA]].
+          rewrite (state_to_list_dead dA)/= => SB.
+          rewrite (HB _ _ _ sB vB SB)//.
+        have [y[ys H]]:= failed_state_to_list vA (success_failed _ sA) (state_to_list B l ++ l).
+        rewrite H/= => bB[?]/cats20[]; destruct ys => //_ SB; subst.
+        rewrite (HA _ _ _ sA vA H).
+        have vB := bbOr_valid bB.
+        move: bB.
+        rewrite /bbOr => /orP[] bB; last first.
+          rewrite next_alt_aux_base_or_ko//if_same//.
+        have [x[xs]]:= failed_state_to_list vB (base_or_failed bB) l.
+        rewrite SB//.
+      - move=> A HA B0 _ B HB l x s/=/andP[sA sB]/and3P[vA].
+        rewrite sA/==> vB bB0.
+        have [y[ys H1]]:= failed_state_to_list vA (success_failed _ sA) l.
+        have [w[ws H2]]:= failed_state_to_list vB (success_failed _ sB) l.
+        rewrite H1 H2/= => -[?]/cats20[]; subst.
+        destruct ws => //=.
+        rewrite (success_is_dead sA) (success_failed _ sA) (HB _ _ _ sB vB H2).
+        move: bB0; rewrite /bbAnd => /orP[] H.
+          have [z[zs sB0]]:= base_and_state_to_list H l.
+          rewrite sB0/=; destruct ys => //.
+          rewrite (HA _ _ _ sA vA H1)//.
+        rewrite (base_and_ko_failed H).
+        case: next_alt => [[]|]//.
+    Qed.
+
+    Lemma state_to_list_empty_next_alt {B l s2}:
+      valid_state B -> state_to_list B l = [::] ->  next_alt s2 B = None.
+    Proof.
+      elim: B l s2 => //.
+      - move=> p[]//.
+      - move=> A HA s B HB l s2/= + /cats20[+ sB].
+        rewrite sB/=.
+        case sA: state_to_list => //.
+        case: ifP => //[dA vB|dA /andP[vA bB]] _.
+          rewrite (HB _ _ vB sB)//.
+        rewrite (HA _ _ vA sA) (HB _ _ (bbOr_valid bB) sB)//if_same//.
+      - move=> A HA B0 _ B HB l s2/=/and3P[vA].
+        case: (ifP (is_dead _)) => //dA.
+        case: ifP => /=[sA vB bB0 | sA /eqP->].
+          have [x[xs H]]:= failed_state_to_list vA (success_failed _ sA) l.
+          rewrite H/==> /cats20[].
+          case sB: state_to_list => // _.
+          rewrite (HB _ _ vB sB) if_same.
+          have vB0 := bbAnd_valid bB0.
+          move: bB0; rewrite /bbAnd => /orP[] bB0; last first.
+            rewrite base_and_ko_failed//; case: next_alt => [[]|]//.
+          have [y [ys sB0]] := failed_state_to_list vB0 (base_and_failed bB0) l.
+          rewrite sB0/=; case: xs H => //= H.
+          by have -> := success_success_singleton_next_alt sA vA H.
+        case SA: (state_to_list A) => /= [|x xs].
+          rewrite (HA _ _ vA SA).
+          case: ifP => //fA bB.
+          have [y [ys +]] := failed_state_to_list vA fA l.
+          rewrite SA//.
+        move=> bB /cats20[].
+        have vB : valid_state B.
+          move: bB; case: ifP => //[_/bbAnd_valid|_/base_and_valid]//.
+        case SB: (state_to_list B) => //= _ _.
+        rewrite (HB _ _ vB SB) if_same.
+        case X: next_alt => [[s3 C]|]//.
+        case: ifP => //fB.
+        have [y [ys]]:= failed_state_to_list vB fB l.
+        by rewrite SB.
+    Qed.
+
+    Lemma expand_failure_next_alt_state_to_list_cons {s A B s1 C}:
+      expand s A = Failure B ->
+        next_alt s B = Some (s1, C) -> 
+          valid_state A -> state_to_list_cons C -> state_to_list_cons A.
+    Proof.
+      elim: A s B s1 C => //.
+      - move=> /= ???? [<-]//.
+      - move=> p [|t]//.
+      - move=> A HA s B HB /= s1 C s2 D + + + + l.
+        case: ifP => dA.
+          case X: expand => // [E] [<-]/=; rewrite dA.
+          case Y: next_alt => [[s3 F]|]//[_<-]/=.
+          move=> vB; rewrite (state_to_list_dead dA)//= => H.
+          have {}H: (state_to_list_cons F).
+            move=> l1; have [y[ys]]:= H l1 => /=; rewrite state_to_list_dead//==>->; by do 2 eexists.
+          by have:= HB _ _ _ _ X Y vB H l.
+        case X: expand => //[E][<-]/=; rewrite (expand_not_dead dA X).
+        case Y: next_alt => [[s3 F]|].
+          move=>[_<-]/=/andP[vA bB].
+          case Z: (state_to_list B l); last first.
+            case: state_to_list => /=; by do 2 eexists.
+          rewrite cats0/= => H.
+          have {}H: (state_to_list_cons F).
+            move=> l1; have /=[x[xs]]:= H l1.
+            rewrite (state_to_list_empty_bt Z) cats0/=.
+            case: state_to_list => //y ys; by do 2 eexists.
+          have [y[ys ->]] := HA _ _ _ _ X Y vA H l.
+          by do 2 eexists.
+        case: ifP => dB //.
+        case Z: next_alt => //[[s3 F]][_<-]/=/andP[vA].
+        rewrite /bbOr; case W: base_or_aux_ko.
+          rewrite next_alt_aux_base_or_ko// in Z.
+        rewrite orbF => bB /(_ l)/=.
+        rewrite (state_to_list_dead is_dead_dead)/= (base_or_aux_next_alt_some bB Z).
+        move=> [x[xs ->]]; case: state_to_list => //; by do 2 eexists.
+      - move=> A HA B0 _ B HB s C/= s2 D + + /and3P[vA + +] + l.
+        case X: expand => //[A'|s1 A'].
+          rewrite (expand_not_solved_not_success X erefl) (expand_failure_failed X)/=.
+          move=> [<-]/=+/eqP H bB; subst B0.
+          case: ifP => //dA.
+          rewrite (expand_failure_failed X).
+          case Y: next_alt => //[[s3 E]].
+          case: ifP => //fB[_<-]/=.
+          move: bB; rewrite /bbAnd.
+          case Z:base_and_ko.
+            rewrite base_and_ko_failed// in fB.
+          rewrite orbF => bB.
+          have [x[xs->]]:= base_and_state_to_list bB l => H.
+          have {}H : (state_to_list_cons E).
+            move=> l1; have /=[y[ys]]:= H l1.
+            have [z[zs->]]:= base_and_state_to_list bB l1.
+            case: state_to_list => //; by do 2 eexists.
+          have [y[ys->]]:= HA _ _ _ _ X Y vA H l.
+          by do 2 eexists.
+        case Y: expand => //[B'][<-]/=.
+        have sA := (expand_solved_success X).1.
+        have sA' := (expand_solved_success X).2.
+        rewrite success_is_dead//success_failed//sA/==>+vB bB0.
+        rewrite (expand_solved_state_to_list_same X).
+        have /= [x[xs H]] := failed_state_to_list (valid_state_expand vA X) (success_failed _ sA') l.
+        rewrite H/=.
+        case nB' : next_alt => [[s3 E]|].
+          move=>[_<-]/(_ l)/=.
+          rewrite H/= => //.
+          move=> [y[ys]].
+          case sE: state_to_list => //=[|w ws].
+            move=>->; case: state_to_list ; by do 2 eexists.
+          move=>[?]; subst.
+          have [{}s3 {}nB'] := next_alt_some nB' s1.
+          have SE : state_to_list_cons E.
+            move=> l1.
+            have:= state_to_list_same_size sE erefl => /(_ l1).
+            case: state_to_list => //.
+            by do 2 eexists.
+          have [z[zs ->]]:= HB _ _ _ _ Y nB' vB SE l.
+          by do 2 eexists.
+        case nA': next_alt => [[s3 E]|]//.
+        case: ifP => //fB0[_<-].
+        move: bB0; rewrite/bbAnd => /orP[]; last first.
+          move=>/base_and_ko_failed; rewrite fB0//.
+        move=> bB0.
+        have [y[ys H1]]:= base_and_state_to_list bB0 l.
+        rewrite H1/=.
+        move=>/(_ l)/=; rewrite H1.
+        case sE: state_to_list => //=[|w ws].
+          move=>[?[]]//.
+        move=> [z[zs]] [??]; subst.
+        case SB: state_to_list => //=; try by do 2 eexists.
+        destruct xs => //=; try by do 2 eexists.
+        by rewrite (success_success_singleton_next_alt sA' (valid_state_expand vA X) H) in nA'.
+      Qed.
+
+
+    Lemma runElpi1 A :
+      forall s B s1 b,
+        valid_state A ->
+          runb s A s1 B b -> 
+            state_to_list_cons A.
+    Proof.
+      move=> s B s1 b + H.
+      elim: H; clear.
+      - move=> s s' A B _ b HA _ vA l.
+        apply: expandb_done_state_to_list_cons vA HA _.
+      - move=> s1 s2 _ A B C _ b1 _ _ HA HB _ IH _ vA.
+        have {}IH := IH (valid_state_next_alt (valid_state_expanded vA (ex_intro _ _ HA)) HB).
+        remember (Failed _) as f eqn:Hf.
+        elim: HA s2 B C Hf HB vA IH; clear => //.
+        - move=> s A B HA s1 _ C [<-] HB vA sC.
+          apply: expand_failure_next_alt_state_to_list_cons HA HB vA sC.
+        - move=> s s' r A B b HA HB IH s2 C D? HC vA sD; subst.
+          have [{}s2 {}HC]:= next_alt_some HC s'.
+          have{}IH := IH _ _ _ erefl HC (valid_state_expand vA HA) sD.
+          apply: expand_state_to_list_cons vA HA notF.
+        - move=> s s' r A B b HA HB IH s2 C D? HC vA sD; subst.
+          have [{}s2 {}HC]:= next_alt_some HC s'.
+          have{}IH := IH _ _ _ erefl HC (valid_state_expand vA HA) sD.
+          apply: expand_state_to_list_cons vA HA notF.
+    Qed.
+
+  End list_cons.
   
   (* Goal @runElpi (And OK Bot Bot).
   Proof.
@@ -284,7 +812,7 @@ Module Nur (U : Unif).
       by rewrite HA HB HB0.
   Qed. *)
 
-  Lemma add_ca_compose {x l1 l2}:
+  (* Lemma add_ca_compose {x l1 l2}:
     add_ca x (l1 ++ l2) = add_ca (add_ca x l1) l2.
   Proof. case: x => //= l; rewrite catA//. Qed.
 
@@ -295,260 +823,15 @@ Module Nur (U : Unif).
   Lemma add_cas_compose_map {l l1 l2}:
     [seq add_cas la (l1 ++ l2) | la <- l] =  
       [seq add_cas la l2 | la <- [seq add_cas la l1 | la <- l]].
-  Proof. elim: l => //x xs IH/=; rewrite IH add_cas_compose//. Qed.
+  Proof. elim: l => //x xs IH/=; rewrite IH add_cas_compose//. Qed. *)
 
 
-  Lemma state_to_list_dead {A l}: is_dead A -> state_to_list A l = [::].
-  Proof.
-    elim: A l => //.
-    - move=> A HA s B HB/= l/andP[dA dB].
-      rewrite HB// HA//.
-    - move=> A HA B0 HB0 B HB l /=dA.
-      rewrite HA//=.
-      (* case: A HA dA=> //A1 s A2/= +/=/andP[dA1 dA2].
-      rewrite dA1 dA2 => /(_ l erefl).
-      move=>/cats20[+ H]/=.
-      rewrite H cats0=>/=.
-      case X: state_to_list => //. *)
-  Qed.
-
-  Lemma success_state_to_list {A m}:
-    (* valid_state A -> *)
-    success A ->
-      state_to_list A m = [::] :: (state_to_list (clean_success A) m).
-  Proof.
-    elim: A m => //.
-    - move=> A HA s B HB/= m.
-      case: ifP => [dA sB|dA sA].
-        rewrite (state_to_list_dead dA)/=.
-        have:= HB _ sB=>->.
-        rewrite (state_to_list_dead dA)//=.
-      have:= HA (state_to_list B m ++ m) sA.
-      move=>->//.
-    - move=> A HA B0 HB0 B HB m /=/andP[sA sB].
-      rewrite /add_alt sA=>/=.
-      have:= HA m sA => ->.
-      have:= HB m sB => ->//=.
-  Qed.
-
-  Lemma expand_solved_state_to_list_same {s1 A s2 B l}:
-    expand s1 A = Solved s2 B -> state_to_list A l = state_to_list B l.
-  Proof.
-    elim: A s1 B s2 l => //.
-    - move=> /= ????[_<-]//.
-    - move=>?[]//.
-    - move=> A HA s B HB s1 C s2 l.
-      move=>/simpl_expand_or_solved[].
-        move=>[A'[HA'->]]/=.
-        by rewrite (HA _ _ _ _ HA').
-      move=> [B'[dA[HB' ->]]]/=.
-      rewrite !(state_to_list_dead dA)//=.
-      apply: HB HB'.
-    - move=> A HA B0 _ B HB s1 C s2 l.
-      move=>/simpl_expand_and_solved[s'[A'[B'[HA'[HB'->]]]]]/=.
-      by rewrite (HA _ _ _ _ HA')(HB _ _ _ _ HB').
-  Qed.
-
-  Lemma state_to_list_empty_clean {B l}:
-    success B -> state_to_list B l = [::[::]] ->
-      state_to_list (clean_success B) l = [::].
-  Proof.
-    move=>/success_state_to_list->.
-    by move=>[].
-  Qed.
-
-  Lemma state_to_list_eq_clean {A B l}:
-    success A -> success B -> state_to_list A l = state_to_list B l ->
-      state_to_list (clean_success A) l = state_to_list (clean_success B) l.
-  Proof.
-    move=>/success_state_to_list->.
-    by move=>/success_state_to_list->[].
-  Qed.
-
-  Lemma base_and_state_to_list {A}: base_and A -> state_to_list_cons A.
-  Proof.
-    elim: A => //=.
-    - by do 2 eexists.
-    - move=> []//p [|t]//= _ B0 _ B HB/andP[/eqP->/HB] H l; have[x[xs]]:= H l => /=->; by do 2 eexists.
-  Qed.
-
-  Lemma base_and_ko_state_to_list {A l}: base_and_ko A -> state_to_list A l = [::].
-  Proof. elim: A => //=-[]//. Qed.
-
-  Lemma base_or_aux_ko_state_to_list {A l}: base_or_aux_ko A -> state_to_list A l = [::].
-  Proof.
-    elim: A l => //.
-    - move=> /= A HA s B HB l /andP[bA bB]; rewrite HB//=base_and_ko_state_to_list//.
-    - move=>[]//.
-  Qed.
-
-  Lemma failed_state_to_list {A}:
-    valid_state A -> failed A = false -> state_to_list_cons A.
-  Proof.
-    elim: A => //.
-    - move=> /=. by move=> /=; do 2 eexists.
-    - by move=> /=; do 2 eexists.
-    - by move=> p []//=; do 2 eexists.
-    - move=> A HA s B HB/=++l.
-      case: ifP => [dA vB fB|dA /andP[vA bB] fA]/=.
-        rewrite (state_to_list_dead dA).
-        apply: HB => //.
-      have [x[xs ->]] := HA vA fA (state_to_list B l ++ l).
-      by do 2 eexists.
-    - move=> A HA B0 _ B HB/= /and3P[]++++l/=.
-      case: ifP => [sA vA vB bB0|sA vA/eqP->]/=.
-        rewrite success_failed//==>fB.
-        rewrite (success_state_to_list sA)/=.
-        have [x[xs]]:= HB vB fB l.
-        move=>->/=; by do 2 eexists.
-      rewrite orbF => + fA; rewrite fA => bB.
-      have [x[xs ->]]:= HA vA fA l.
-      have [y[ys ->]]:= base_and_state_to_list bB l.
-      by do 2 eexists.
-  Qed.
-
-  Lemma expandedb_done_state_to_list {A s B s1 b}:
-    valid_state A -> expandedb s A (Done s1 B) b ->
-      state_to_list_cons A.
-  Proof.
-    move=>+/expandedb_Done_not_failed.
-    apply: failed_state_to_list.
-  Qed.
-
-  Lemma next_alt_state_to_list_old {s1 A s2 B}:
-    valid_state A -> next_alt s1 A = Some (s2, B) -> state_to_list_cons B.
-  Proof.
-    move=>vA H.
-    have:= next_alt_failed H.
-    have:= valid_state_next_alt vA H.
-    apply: failed_state_to_list.
-  Qed.
-
-  Lemma success_next_alt_state_to_list {s1 A}:
-    valid_state A -> success A -> next_alt s1 A = None -> 
-      forall l, exists x, state_to_list A l = [::x].
-  Proof.
-    elim: A s1 => //.
-    - by exists [::].
-    - move=> A HA s B HB s1/=.
-      case: ifP => [dA vB sB|dA /andP[vA bB] sA] + l.
-        rewrite state_to_list_dead//=.
-        case X: next_alt => [[]|]// _.
-        by have:= HB _ vB sB X l.
-      case X: next_alt => [[]|]//.
-      have H:= bbOr_valid bB.
-      case: ifP => dB.
-        rewrite valid_state_dead// in H.
-      (* case: ifP => // fB. *)
-      case Y: next_alt => [[]|]// _.
-      have [x H1] := HA _ vA sA X (state_to_list B l ++ l).
-      rewrite H1/=.
-      have:= bB; rewrite /bbOr.
-      case Z: base_or_aux => //=.
-        have H2 := next_alt_aux_base_or_none Z Y.
-        by subst.
-      move=> bB0'.
-      rewrite (base_or_aux_ko_state_to_list bB0')/=.
-      by eexists.
-    - move=> A HA B0 _ B HB s1 /=/and3P[vA].
-      case: ifP => //sA vB/=bB0 sB + l.
-      rewrite success_is_dead// success_failed//.
-      case X: next_alt => [[]|]//.
-      have [x H1] := HB _ vB sB X l; rewrite H1.
-      case Y: next_alt => [[s2 C]|]//.
-        move: bB0; rewrite /bbAnd.
-        case Z: base_and => //=.
-          rewrite base_and_failed//.
-        move=> bB0; rewrite base_and_ko_failed//base_and_ko_state_to_list/add_alt//=.
-        rewrite success_state_to_list//flatten_empty.
-        by eexists.
-      have [y H2] := HA _ vA sA Y l.
-      rewrite H2/=; by eexists.
-  Qed.
-
-  Lemma bbOr_next_alt_none {s B l}:
-     bbOr B -> next_alt s B = None -> state_to_list B l = [::].
-  Proof.
-    elim: B s l => //.
-    - move=> A HA s B HB s1 l/=; rewrite /bbOr/=.
-      move=>/orP[]/andP[bA bB].
-        rewrite base_and_dead// next_alt_aux_base_and//.
-      rewrite base_and_ko_is_dead// base_or_aux_is_dead//.
-      have H1 := @next_alt_aux_base_or_ko _ s bB.
-      have H2 :=  @next_alt_aux_base_and_ko _ s1 bA.
-      rewrite (HA _ _ _ H2)// ?(HB _ _ _ H1)///bbOr ?bB?orbT//base_and_ko_base_or_aux_ko//orbT//.
-    - move=> []//p a _ B0 _ B HB s l/=; rewrite /bbOr/=orbF => /andP[/eqP->bB].
-      rewrite next_alt_aux_base_and//.
-  Qed.
-
-  Lemma base_or_aux_next_alt_some {s B s1 D l}:
-     base_or_aux B -> next_alt s B = Some (s1, D) -> state_to_list B l = state_to_list D l.
-  Proof.
-    elim: B s s1 D l => //.
-    - move=>/=???? _[_<-]//.
-    - move=> A HA s B HB s1 s3 C l/=/andP[bA bB].
-      rewrite base_and_dead//next_alt_aux_base_and//.
-      move=>[_<-]//.
-    - move=> []// p a _ B0 _ B HB s1 s2 C l/=/andP[/eqP->bB].
-      rewrite next_alt_aux_base_and// => -[_<-]//.
-  Qed.
-
-
-  Lemma failed_next_alt_state_to_list {s1 A}:
-    valid_state A -> failed A -> next_alt s1 A = None -> 
-      forall l, state_to_list A l = [::].
-  Proof.
-    elim: A s1 => //.
-    - move=> A HA s B HB s1 /=.
-      case: ifP => [dA vB fB|dA /andP[vA bB] fA].
-        case X: next_alt => [[s2 C]|]//.
-        move=> _ l; rewrite (HB s1)//= state_to_list_dead//.
-      case X: next_alt => [[s2 C]|]//.
-      case: ifP => dB.
-        move=>_ l; rewrite (HA s1)//state_to_list_dead//.
-      (* case: ifP => fB//. *)
-      case Y: next_alt => [[]|]// _ l.
-      rewrite (HA s1)//=.
-      rewrite (bbOr_next_alt_none bB Y)//.
-    - move=> A HA B0 HB0 B HB s1/=/and3P[vA].
-      case: ifP => /=[sA vB bB0|sA/eqP->].
-        rewrite success_failed//=success_is_dead// => fB.
-        case X: next_alt => [[]|]//.
-        case Y: next_alt => [[s2 C]|]//.
-          case: ifP => fB0// _ l.
-          rewrite (HB s1)//.
-          have:= bB0; rewrite /bbAnd.
-          case Z: base_and => //=.
-            rewrite base_and_failed// in fB0.
-          move=> bB0'.
-          have H := @next_alt_aux_base_and_ko _ empty bB0'.
-          have H1:= bbAnd_valid bB0.
-          rewrite (HB0 empty)/add_alt//=; case: state_to_list => //*; rewrite flatten_empty//.
-        move=> _ l.
-        have [x H]:= success_next_alt_state_to_list vA sA Y l.
-        rewrite H.
-        rewrite (HB s1)/add_alt//=.
-      case: ifP => //fA bB _ + l.
-      case: ifP => //dA.
-        rewrite (state_to_list_dead dA)//.
-      case X: next_alt => [[s2 C]|].
-        case:ifP => fB => //.
-        have:= bB; rewrite /bbAnd.
-        case Z: base_and => //=.
-          rewrite base_and_failed// in fB.
-        move=> bB0'.
-        have H := @next_alt_aux_base_and_ko _ empty bB0'.
-        have H1:= bbAnd_valid bB.
-        rewrite (HB empty)/add_alt//=; case: state_to_list => //*; rewrite flatten_empty//.
-      have -> //:= HA _ vA fA X l.
-  Qed.  
-
-  Lemma next_alt_state_to_list {s1 A s2 B}:
-    valid_state A -> next_alt s1 A = Some (s2, B) -> 
-      forall l, state_to_list A l = state_to_list B l.
+  (* Lemma next_alt_state_to_list {s1 A s2 B}:
+    valid_state A -> failed A -> next_alt s1 A = Some (s2, B) -> 
+      forall l, exists x, state_to_list A l = x :: state_to_list B l.
   Proof.
     elim: A s1 s2 B  => //.
-    - move=>/=??? _ [_<-]//.
+    - move=>/=??? _ [_<-]//?; exists [::]. => /=.
     - move=>/=????? _ [_<-]//.
     - move=> A HA s B HB s1 s2 C/=.
       case: ifP => //[dA vB | dA /andP[vA bB]].
@@ -633,7 +916,7 @@ Module Nur (U : Unif).
         have H1:= bbAnd_valid bB0.
         have:= 
 
-  Qed.
+  Qed. *)
 
   Lemma next_alt_state_to_list {s1 A s2 B}:
     valid_state A -> failed A -> next_alt s1 A = Some (s2, B) -> 
@@ -652,6 +935,10 @@ Module Nur (U : Unif).
       case: ifP => //dB.
       case Y: next_alt => [[s3 D]|]//[_<-]/= l.
       rewrite (state_to_list_dead is_dead_dead)/= (failed_next_alt_state_to_list vA fA X)/=.
+      move: bB; rewrite /bbOr.
+      case Z: (base_or_aux_ko B).
+        rewrite next_alt_aux_base_or_ko// in Y.
+      rewrite orbF.
       admit.
     - move=> A HA B0 HB0 B HB s1 s2 C/=/and3P[vA].
       case: ifP => /=[sA vB bB0|sA /eqP/[dup]H->].
@@ -672,7 +959,7 @@ Module Nur (U : Unif).
         have H := @next_alt_aux_base_and _ empty bB0'.
         have H1:= bbAnd_valid bB0.
 
-  Qed.
+  Abort.
 
 
   Lemma expandedb_fail_state_to_list {s A B b1 s' C}:
@@ -702,10 +989,7 @@ Module Nur (U : Unif).
             rewrite H/=.
             by eexists.
           case: ifP => //dB.
-          case: ifP => //fB.
-            case Z: next_alt => [[s4 G]|]//[_<-]/=.
-            rewrite (state_to_list_dead is_dead_dead)/=.
-
+        Abort.
     
   
 
@@ -745,7 +1029,7 @@ Module Nur (U : Unif).
     expand s A = Solved s1 B ->
       forall l,
         exists r1,
-          (nur' r1 A l s s1) /\ state_to_list (clean_success B) l = r1.
+          (nur' A l s s1 r1) /\ state_to_list (clean_success B) l = r1.
   Proof.
     move=> H l .
     have [sA sB] := expand_solved_success H.
@@ -762,28 +1046,29 @@ Module Nur (U : Unif).
 
   Lemma runExpandedbDone {s s' A B b}:
     expandedb s A (Done s' B) b ->
+    valid_state A ->
     forall l,
       exists r1,
-        (nur' r1 A l s s') /\ state_to_list (clean_success B) l = r1.
+        (nur' A l s s' r1) /\ state_to_list (clean_success B) l = r1.
   Proof.
     remember (Done _ _) as d eqn:Hd => H.
     elim: H s' B Hd => //; clear.
-    - move=> s s' A A' + s1 B [??]; subst.
+    - move=> s s' A A' + s1 B [??] _; subst.
       apply: expand_done.
-    - move=> s s' r A B b H1 H2 IH s1 C ? l; subst.
-      have {IH} := IH _ _ erefl l.
+    - move=> s s' r A B b H1 H2 IH s1 C ? vA l; subst.
+      have {IH} := IH _ _ erefl (valid_state_expand vA H1) l.
       rewrite /nur'.
       move=> [r1 [H3 H4]].
-      have [x [xs]] := expandedb_done_state_to_list H2 l.
+      have [x [xs]] := expandedb_done_state_to_list (valid_state_expand vA H1) H2 l.
       move=>{}/H3 H3.
       exists r1; split => // w ws H p.
       have {}H3 := H3 p.
       admit.
-    - move=> s s' r A B b H1 H2 IH s1 C ? l; subst.
-      have {IH} := IH _ _ erefl l.
+    - move=> s s' r A B b H1 H2 IH s1 C ? vA l; subst.
+      have {IH} := IH _ _ erefl (valid_state_expand vA H1) l.
       rewrite /nur'.
       move=> [r1 [H3 H4]].
-      have [x [xs]] := expandedb_done_state_to_list H2 l.
+      have [x [xs]] := expandedb_done_state_to_list (valid_state_expand vA H1) H2 l.
       move=>{}/H3 H3.
       exists r1; split => // w ws H p.
       have {}H3 := H3 p.
@@ -797,41 +1082,26 @@ Module Nur (U : Unif).
   Admitted.
 
   Lemma rrrr {s A B s' C l x xs}:
-    expand s A = Failure B ->
+    expand s A = Failure B -> valid_state A ->
       next_alt s B = Some (s', C) -> state_to_list A l = x :: xs -> state_to_list C l = xs.
   Proof.
     elim: A s B s' C l x xs => //.
-    - move=> s B s' C l x xs[<-]//.
+    (* - move=> s B s' C l x xs[<-]//. *)
     - move=> p [|t]//.
-    - move=> A HA s B HB s1 C s2 D l x xs.
-      move=>/simpl_expand_or_fail[].
-        move=>[A'[dA[HA'->]]]/=; clear HB.
-        have /= dA':= expand_not_dead dA HA'.
-        case: ifP => /eqP// _.
-        case X: next_alt => [[s3 E]|].
-          move=>[_<-]/=.
-          case Y: state_to_list => [|y ys].
-            admit.
-          have:= HA _ _ _ _ _ _ _ HA' X Y.
-          by move=>->[].
-        case: ifP => /eqP//dB.
-        case: ifP => fB//.
-          case: next_alt => [[s3 E]|]//.
-          move=>[_<-]/=.
-          rewrite state_to_list_dead/=.
-          case Y: state_to_list => [|y ys]/=.
-            admit.
-          move=>[] _ H.
+    - move=> A HA s B HB s1 C s2 D l x xs/=.
+      case: ifP => dA.
+        rewrite state_to_list_dead//=.
+        case X: expand => //[B'][?]; subst.
 
-      move=>
 
   Lemma zzzz {s A B b1 l x xs s' C}:
+    valid_state A ->
     expandedb s A (Failed B) b1 ->
       next_alt s B = Some (s', C) ->
         state_to_list A l = x :: xs ->
           state_to_list C l = xs.
   Proof.
-    remember (Failed _) as f eqn:Hf => H.
+    remember (Failed _) as f eqn:Hf => +H.
     elim: H B l x xs s' C Hf; clear => //.
     - move=> s A B + ? l x xs s' C[<-].
       clear.
@@ -843,16 +1113,18 @@ Module Nur (U : Unif).
 
   Lemma runElpiP: forall A, runElpi A.
   Proof.
-    move=> A s B s1 b H.
+    move=> A s B s1 b + H.
     elim: H; clear.
     + move=>  s s' A B C b + ->/=.
       apply: runExpandedbDone.
-    + move=> s s' s2 A B C D b1 b2 b3 HA HB HC IH ? l; subst.
-      have {IH} := IH l.
+    + move=> s s' s2 A B C D b1 b2 b3 HA HB HC IH ? vA l; subst.
+      have vB := valid_state_expanded vA (ex_intro _ _ HA).
+      have vC := valid_state_next_alt vB HB.
+      have {IH} := IH vC l.
       rewrite /nur'.
       move=> [r1 [H1 H2]].
       exists r1; split => // x xs H p.
-      have:= next_alt_state_to_list HB.
+      have:= next_alt_state_to_list_old vB HB.
       move=> /(_ l) [y [ys H3]].
       have {}H1:= H1 _ _ H3 p.
       rewrite /state_to_list_cons.
